work on PackedKV

lib/DataStructures/PackedKV.i.dfy
@@ -1,8 +1,16 @@
 include "PackedStringArray.i.dfy"
 include "../Base/total_order.i.dfy"
+include "../../ByteBlockCacheSystem/KVList.i.dfy"
 
 module PackedKV {
+  import PackedStringArray
+  import KVList
+  import opened NativeTypes
   import Keyspace = Lexicographic_Byte_Order
+  import opened KeyType
+  import opened ValueType`Internal
+  import opened ValueMessage
+  import opened BucketsLib
 
   datatype Pkv = Pkv(
       keys: PackedStringArray.Psa,
@@ -10,24 +18,118 @@ module PackedKV {
 
   predicate ValidKeyByteString(s: seq<byte>)
   {
-    |s| <= KeyType.MaxLen()
+    |s| <= KeyType.MaxLen() as int
   }
 
   predicate ValidMessageByteString(s: seq<byte>)
   {
-    |s| <= ValueWithDefault.MaxLen()
+    |s| <= ValueType.MaxLen() as int
   }
 
   predicate ValidKeyLens(psa: PackedStringArray.Psa)
+  requires PackedStringArray.WF(psa)
   {
     forall i | 0 <= i < |psa.offsets| ::
-        PackedStringArray.psaEnd(psa, i) - PackedStringArray.psaStart(psa, i) <= KeyType.MaxLen()
+        PackedStringArray.psaEnd(psa, i) as int - PackedStringArray.psaStart(psa, i) as int <= KeyType.MaxLen() as int
   }
 
   predicate WF(pkv: Pkv) {
     && PackedStringArray.WF(pkv.keys)
     && PackedStringArray.WF(pkv.values)
     && ValidKeyLens(pkv.keys)
-    && ValidMessageLens(pkv.messages)
+    && |pkv.keys.offsets| == |pkv.values.offsets|
+  }
+
+  function {:opaque} psaSeq_Keys(psa: PackedStringArray.Psa, i: int) : (res : seq<Key>)
+  requires PackedStringArray.WF(psa)
+  requires ValidKeyLens(psa)
+  requires 0 <= i <= |psa.offsets|
+  ensures |res| == i
+  ensures forall j | 0 <= j < i :: res[j] == PackedStringArray.psaElement(psa, j)
+  {
+    if i == 0 then [] else psaSeq_Keys(psa, i-1) + [PackedStringArray.psaElement(psa, i-1)]
+  }
+
+  function IKeys(psa: PackedStringArray.Psa) : (res : seq<Key>)
+  requires PackedStringArray.WF(psa)
+  requires ValidKeyLens(psa)
+  {
+    psaSeq_Keys(psa, |psa.offsets|)
+  }
+
+  function method byteString_to_Message(s: seq<byte>) : Message
+  requires |s| < 0x1_0000_0000
+  {
+    if |s| as uint64 <= ValueType.MaxLen() then (
+      Define(s)
+    ) else (
+      // NOTE(travis)
+      // It's just convenient to make this function total, so
+      // we just do this if the byte string is invalid.
+      Define(ValueType.DefaultValue())
+    )
+  }
+
+  function {:opaque} psaSeq_Messages(psa: PackedStringArray.Psa, i: int) : (res : seq<Message>)
+  requires PackedStringArray.WF(psa)
+  requires 0 <= i <= |psa.offsets|
+  ensures |res| == i
+  ensures forall j | 0 <= j < i :: res[j] == byteString_to_Message(PackedStringArray.psaElement(psa, j))
+  {
+    if i == 0 then [] else psaSeq_Messages(psa, i-1) + [
+        byteString_to_Message(PackedStringArray.psaElement(psa, i-1))]
+  }
+
+  function IMessages(psa: PackedStringArray.Psa) : (res : seq<Message>)
+  requires PackedStringArray.WF(psa)
+  {
+    psaSeq_Messages(psa, |psa.offsets|)
+  }
+
+  function Imap(pkv: Pkv, i: int) : (bucket : Bucket)
+  requires WF(pkv)
+  requires 0 <= i <= |pkv.keys.offsets|
+  ensures WFBucket(bucket)
+  {
+    reveal_WFBucket();
+
+    if i == 0 then map[] else (
+      var key : Key := PackedStringArray.psaElement(pkv.keys, i-1);
+      var msg : Message := byteString_to_Message(PackedStringArray.psaElement(pkv.keys, i-1));
+      Imap(pkv, i-1)[key := msg]
+    )
+  }
+
+  function I(pkv: Pkv) : (bucket : Bucket)
+  requires WF(pkv)
+  ensures WFBucket(bucket)
+  {
+    Imap(pkv, |pkv.keys.offsets|)
+  }
+
+  method ComputeValidKeyLens(psa: PackedStringArray.Psa)
+  returns (b: bool)
+  requires PackedStringArray.WF(psa)
+  ensures b == ValidKeyLens(psa)
+  {
+    assume false; 
+
+    if |psa.offsets| as uint64 == 0 {
+      return true;
+    }
+    if psa.offsets[0 as uint64] as uint64 > KeyType.MaxLen() {
+      return false;
+    }
+
+    var i: uint64 := 1;
+    while i < |psa.offsets| as uint64
+    {
+      if psa.offsets[i] as uint64 - psa.offsets[i-1] as uint64 > KeyType.MaxLen() {
+        return false;
+      }
+      i := i + 1;
+    }
+
+    return true;
   }
 }
